theories/int_or_ptr/vst/spec/spec.v
@@ -2,8 +2,36 @@ From VST Require Import floyd.proofauto.
 
 From appliedfm Require Import int_or_ptr.model.int_or_ptr.
 From appliedfm Require Import int_or_ptr.vst.ast.ast.
+From appliedfm Require Import int_or_ptr.vst.cmodel.constants.
 From appliedfm Require Import int_or_ptr.vst.cmodel.val.
 From appliedfm Require Import int_or_ptr.vst.clightgen.int_or_ptr.
+
+
+Definition int_or_ptr__sizeof_spec :=
+ DECLARE _int_or_ptr__sizeof
+ WITH u : unit
+ PRE [ ]
+   PROP ()
+   PARAMS ()
+   GLOBALS ()
+   SEP ()
+ POST [ (if Archi.ptr64 then tulong else tuint) ]
+   PROP()
+   LOCAL(temp ret_temp (if Archi.ptr64 then Vlong (Int64.repr word_size) else Vint (Int.repr word_size)))
+   SEP().
+
+Definition int_or_ptr__alignof_spec :=
+ DECLARE _int_or_ptr__alignof
+ WITH u : unit
+ PRE [ ]
+   PROP ()
+   PARAMS ()
+   GLOBALS ()
+   SEP ()
+ POST [ (if Archi.ptr64 then tulong else tuint) ]
+   PROP()
+   LOCAL(temp ret_temp (if Archi.ptr64 then Vlong (Int64.repr (Z.shiftl 1 word_align)) else Vint (Int.repr (Z.shiftl 1 word_align))))
+   SEP().
 
 Definition int_or_ptr__is_int_spec :=
  DECLARE _int_or_ptr__is_int
@@ -71,7 +99,9 @@ Definition int_or_ptr__of_ptr_spec :=
     SEP().
 
 Definition ASI: funspecs := ltac:(with_library prog
-  [ int_or_ptr__is_int_spec
+  [ int_or_ptr__sizeof_spec
+  ; int_or_ptr__alignof_spec
+  ; int_or_ptr__is_int_spec
   ; int_or_ptr__to_int_spec
   ; int_or_ptr__to_ptr_spec
   ; int_or_ptr__of_int_spec
