theories/int_or_ptr/model/int_or_ptr.v
@@ -1,0 +1,3 @@
+From Coq Require Import ZArith.ZArith.
+
+Definition int_or_ptr (X: Type): Type := option (Z + X).
