theories/int_or_ptr/vst/cmodel/constants.v
@@ -1,0 +1,5 @@
+From VST Require Import floyd.proofauto.
+
+Definition word_size: Z := Eval cbv [Archi.ptr64] in if Archi.ptr64 then 8 else 4.
+
+Definition word_align: Z := Eval cbv [Archi.ptr64] in if Archi.ptr64 then 3 else 2.
